src/lib/extraction/BvUtil.ml
@@ -1,0 +1,59 @@
+open BinNat
+open BinPos
+open Datatypes
+open Nat0
+open Definitions
+
+module BoolList =
+ struct
+  (** val add_lsb :
+      bool -> Big_int_Z.big_int option -> Big_int_Z.big_int option **)
+
+  let add_lsb b prefix =
+    if b
+    then (match prefix with
+          | Some n ->
+            Some
+              ((fun x -> Big_int_Z.succ_big_int (Big_int_Z.mult_int_big_int 2 x))
+              n)
+          | None -> Some Big_int_Z.unit_big_int)
+    else (match prefix with
+          | Some n -> Some (Big_int_Z.mult_int_big_int 2 n)
+          | None -> None)
+
+  (** val bits_to_N :
+      bool list -> Big_int_Z.big_int option -> Big_int_Z.big_int **)
+
+  let rec bits_to_N x acc =
+    match x with
+    | [] -> (match acc with
+             | Some n -> n
+             | None -> Big_int_Z.zero_big_int)
+    | b :: x0 -> bits_to_N x0 (add_lsb b acc)
+
+  (** val to_Z_unsigned :
+      bool list -> Big_int_Z.big_int option -> Big_int_Z.big_int **)
+
+  let to_Z_unsigned x prefix =
+    (fun fO fp n -> if Big_int_Z.sign_big_int n <= 0 then fO () else fp n)
+      (fun _ -> Big_int_Z.zero_big_int)
+      (fun n -> n)
+      (bits_to_N x prefix)
+
+  (** val prefix_size : Big_int_Z.big_int option -> Big_int_Z.big_int **)
+
+  let prefix_size = function
+  | Some p -> Pos.size_nat p
+  | None -> Big_int_Z.zero_big_int
+
+  (** val to_bv' : bool list -> Big_int_Z.big_int option -> bv **)
+
+  let to_bv' x prefix =
+    coq_Z_to_bv (N.of_nat (add (prefix_size prefix) (length x)))
+      (to_Z_unsigned x prefix)
+
+  (** val to_bv : bool list -> bv **)
+
+  let to_bv x =
+    to_bv' x None
+ end
