src/lib/extraction/BvUtil.mli
@@ -1,0 +1,21 @@
+open BinNat
+open BinPos
+open Datatypes
+open Nat0
+open Definitions
+
+module BoolList :
+ sig
+  val add_lsb : bool -> Big_int_Z.big_int option -> Big_int_Z.big_int option
+
+  val bits_to_N : bool list -> Big_int_Z.big_int option -> Big_int_Z.big_int
+
+  val to_Z_unsigned :
+    bool list -> Big_int_Z.big_int option -> Big_int_Z.big_int
+
+  val prefix_size : Big_int_Z.big_int option -> Big_int_Z.big_int
+
+  val to_bv' : bool list -> Big_int_Z.big_int option -> bv
+
+  val to_bv : bool list -> bv
+ end
