src/lib/extraction/Interval.mli
@@ -3,6 +3,8 @@ open Datatypes
 open OptionUtil
 open Specif
 open ZArith_dec
+open Base
+open Option
 
 module Dom :
  sig
@@ -42,4 +44,63 @@ module Dom :
   val leb : interval -> interval -> bool
 
   val _UU03b1_ : Big_int_Z.big_int -> interval
+
+  val negate_endpoints :
+    (Big_int_Z.big_int option * Big_int_Z.big_int option) ->
+    Big_int_Z.big_int option * Big_int_Z.big_int option
+
+  val negate : interval -> interval
+
+  val add_endpoints :
+    (Big_int_Z.big_int option * Big_int_Z.big_int option) ->
+    (Big_int_Z.big_int option * Big_int_Z.big_int option) ->
+    Big_int_Z.big_int option * Big_int_Z.big_int option
+
+  val add : interval -> interval -> interval
+
+  val sub : interval -> interval -> interval
+
+  val four_corner_endpoints :
+    (Big_int_Z.big_int -> Big_int_Z.big_int -> Big_int_Z.big_int) ->
+    (Big_int_Z.big_int option * Big_int_Z.big_int option) ->
+    (Big_int_Z.big_int option * Big_int_Z.big_int option) ->
+    Big_int_Z.big_int option * Big_int_Z.big_int option
+
+  val lift_binop :
+    (Big_int_Z.big_int -> Big_int_Z.big_int -> Big_int_Z.big_int) -> interval
+    -> interval -> interval
+
+  val mult : interval -> interval -> interval
+
+  val max_endpoints :
+    (Big_int_Z.big_int option * Big_int_Z.big_int option) ->
+    (Big_int_Z.big_int option * Big_int_Z.big_int option) ->
+    Big_int_Z.big_int option * Big_int_Z.big_int option
+
+  val max : interval -> interval -> interval
+
+  val min_endpoints :
+    (Big_int_Z.big_int option * Big_int_Z.big_int option) ->
+    (Big_int_Z.big_int option * Big_int_Z.big_int option) ->
+    Big_int_Z.big_int option * Big_int_Z.big_int option
+
+  val min : interval -> interval -> interval
+
+  val abs_endpoint :
+    (Big_int_Z.big_int option * Big_int_Z.big_int option) ->
+    Big_int_Z.big_int option * Big_int_Z.big_int option
+
+  val abs : interval -> interval
+
+  val tdiv : interval -> interval -> interval
+
+  val tmod : interval -> interval -> interval
+
+  val fdiv : interval -> interval -> interval
+
+  val fmod : interval -> interval -> interval
+
+  val ediv : interval -> interval -> interval
+
+  val emod : interval -> interval -> interval
  end
