src/lib/extraction/ListDef.mli
@@ -1,4 +1,6 @@
 
 val map : ('a1 -> 'a2) -> 'a1 list -> 'a2 list
 
+val seq : Big_int_Z.big_int -> Big_int_Z.big_int -> Big_int_Z.big_int list
+
 val repeat : 'a1 -> Big_int_Z.big_int -> 'a1 list
