src/lib/extraction/list_monad.ml
@@ -1,0 +1,11 @@
+
+type __ = Obj.t
+
+module Coq_list =
+ struct
+  (** val list_fmap : (__ -> __) -> __ list -> __ list **)
+
+  let rec list_fmap f = function
+  | [] -> []
+  | x :: l0 -> (f x) :: (list_fmap f l0)
+ end
