src/lib/extraction/list_monad.mli
@@ -1,0 +1,7 @@
+
+type __ = Obj.t
+
+module Coq_list :
+ sig
+  val list_fmap : (__ -> __) -> __ list -> __ list
+ end
