src/lib/extraction/list_numbers.ml
@@ -1,0 +1,15 @@
+open BinInt
+open ListDef
+open Base
+open List_monad
+
+module Coq_list =
+ struct
+  (** val seqZ :
+      Big_int_Z.big_int -> Big_int_Z.big_int -> Big_int_Z.big_int list **)
+
+  let seqZ m len =
+    fmap (Obj.magic (fun _ _ -> Coq_list.list_fmap)) (fun i ->
+      Z.add (Z.of_nat i) m)
+      (Obj.magic seq Big_int_Z.zero_big_int (Z.to_nat len))
+ end
