src/lib/extraction/list_numbers.mli
@@ -1,0 +1,9 @@
+open BinInt
+open ListDef
+open Base
+open List_monad
+
+module Coq_list :
+ sig
+  val seqZ : Big_int_Z.big_int -> Big_int_Z.big_int -> Big_int_Z.big_int list
+ end
