src/rocq/lib/BvUtil.v
@@ -1,0 +1,449 @@
+(* ************************************************************************ *)
+(*  Sail and the Sail architecture models here, comprising all files and    *)
+(*  directories except the ASL-derived Sail code in the aarch64 directory,  *)
+(*  are subject to the BSD two-clause licence below.                        *)
+(*                                                                          *)
+(*  The ASL derived parts of the ARMv8.3 specification in                   *)
+(*  aarch64/no_vector and aarch64/full are copyright ARM Ltd.               *)
+(*                                                                          *)
+(*  Copyright (c) 2013-2026                                                 *)
+(*    Kathyrn Gray                                                          *)
+(*    Shaked Flur                                                           *)
+(*    Stephen Kell                                                          *)
+(*    Gabriel Kerneis                                                       *)
+(*    Robert Norton-Wright                                                  *)
+(*    Christopher Pulte                                                     *)
+(*    Peter Sewell                                                          *)
+(*    Alasdair Armstrong                                                    *)
+(*    Brian Campbell                                                        *)
+(*    Thomas Bauereiss                                                      *)
+(*    Anthony Fox                                                           *)
+(*    Jon French                                                            *)
+(*    Dominic Mulligan                                                      *)
+(*    Stephen Kell                                                          *)
+(*    Mark Wassell                                                          *)
+(*    Alastair Reid (Arm Ltd)                                               *)
+(*                                                                          *)
+(*  All rights reserved.                                                    *)
+(*                                                                          *)
+(*  This work was partially supported by EPSRC grant EP/K008528/1 REMS:     *)
+(*  Rigorous Engineering for Mainstream Systems, an ARM iCASE award, EPSRC  *)
+(*  IAA KTF funding, and donations from Arm. This project has received      *)
+(*  funding from the European Research Council (ERC) under the European     *)
+(*  Union's Horizon 2020 research and innovation programme (grant agreement *)
+(*  No 789108, ELVER).                                                      *)
+(*                                                                          *)
+(*  This software was developed by SRI International and the University of  *)
+(*  Cambridge Computer Laboratory (Department of Computer Science and       *)
+(*  Technology) under DARPA/AFRL contracts FA8650-18-C-7809 ("CIFV")        *)
+(*  and FA8750-10-C-0237 ("CTSRD").                                         *)
+(*                                                                          *)
+(*  SPDX-License-Identifier: BSD-2-Clause                                   *)
+(* ************************************************************************ *)
+
+(** This file contains extra lemmas about stdpp bitvectors. *)
+
+From stdpp Require Import base.
+From stdpp Require Import bitvector.definitions.
+From stdpp Require Import bitvector.tactics.
+From stdpp Require Import list.
+
+From Sail Require Import Tactics.
+
+Lemma bv_unsigned_log2 : ∀ {n} {x : bv n}, (0 < n)%N → (Z.log2 (bv_unsigned x) < Z.of_N n)%Z.
+Proof.
+  intros n x zero_lt_n.
+  destruct x. unfold BvWf in bv_is_wf.
+  unfold definitions.bv_unsigned.
+  rewrite Is_true_true, andb_true_iff, Z.ltb_lt, Z.leb_le in bv_is_wf.
+  unfold bv_modulus in bv_is_wf.
+  destruct (bv_unsigned =? 0)%Z eqn : E.
+  - rewrite Z.eqb_eq in E.
+    rewrite E.
+    cbn. lia.
+  - apply Z.log2_lt_pow2.
+    + lia.
+    + apply (proj2 bv_is_wf).
+Qed.
+
+Lemma bv_unsigned_nonneg : ∀ {n} {x : bv n}, (0 ≤ bv_unsigned x)%Z.
+Proof.
+  intros n x.
+  destruct x. unfold BvWf in bv_is_wf.
+  unfold definitions.bv_unsigned.
+  rewrite Is_true_true, andb_true_iff, Z.leb_le in bv_is_wf.
+  easy.
+Qed.
+
+Lemma bv_unsigned_shiftl_nonneg : ∀ {n shift} {x : bv n}, (0 ≤ bv_unsigned x ≪ shift)%Z.
+Proof.
+  intros n m x.
+  apply Z.shiftl_nonneg, bv_unsigned_nonneg.
+Qed.
+
+(** We want to show that [bv_to_bits] applied to [bv_concat] can be
+simplified to a list append. This is to let us relate stdpp bitvectors
+and bitlist style bitvectors.
+
+First, we show it for non-empty bitvectors. *)
+
+Lemma bv_concat_app_non_empty : ∀ {n m} {x : bv n} {y : bv m},
+  (0 < n)%N →
+  (0 < m)%N →
+  bv_to_bits (bv_concat (n + m) x y) = bv_to_bits y ++ bv_to_bits x.
+Proof.
+  intros n m x y zero_lt_n zero_lt_m.
+  apply (list_eq_same_length _ _ (N.to_nat (n + m))).
+  - rewrite length_app. repeat rewrite length_bv_to_bits. lia.
+  - rewrite length_bv_to_bits. reflexivity.
+  - intros i lb rb i_lt_n_plus_m L R.
+    rewrite bv_to_bits_lookup_Some in L. destruct L as [_ L].
+    rewrite bv_concat_unsigned', bv_wrap_land in L.
+    rewrite Z.land_ones_low in L; [| shelve | shelve ].
+    rewrite lookup_app_Some in R.
+    repeat rewrite bv_to_bits_lookup_Some in R.
+    rewrite length_bv_to_bits in R.
+    destruct R as [[i_lt_m Ry] | [? [? Rx]]]; subst.
+    + rewrite Z.lor_spec, Z.shiftl_spec_low; [ reflexivity | lia ].
+    + rewrite Z.lor_spec, Z.shiftl_spec_high; try lia.
+      destruct (bv_unsigned y =? 0)%Z eqn : y_zero;
+        [ rewrite Z.eqb_eq in y_zero | rewrite Z.eqb_neq in y_zero].
+      * rewrite y_zero, Z.testbit_0_l, orb_false_r.
+        f_equal. lia.
+      * pattern (Z.testbit (bv_unsigned y) (Z.of_nat i)).
+        rewrite Z.bits_above_log2, orb_false_r; [ f_equal; lia | apply bv_unsigned_nonneg |].
+        apply (Z.lt_le_trans _ _ _ (bv_unsigned_log2 zero_lt_m)). lia.
+    Unshelve.
+    { apply Z.lor_nonneg; split; [ apply bv_unsigned_shiftl_nonneg | apply bv_unsigned_nonneg ]. }
+    { rewrite Z.log2_lor.
+      - apply Z.max_lub_lt.
+        + destruct (bv_unsigned x =? 0)%Z eqn : x_zero. rewrite Z.eqb_eq in x_zero.
+          * rewrite x_zero, Z.shiftl_0_l. cbn. lia.
+          * rewrite Z.log2_shiftl, N2Z.inj_add; try lia.
+            ** apply Z.add_lt_mono_r, (bv_unsigned_log2 (zero_lt_n)).
+            ** rewrite Z.eqb_neq in x_zero. pose proof (@bv_unsigned_nonneg n x). lia.
+        + destruct (bv_unsigned y =? 0)%Z eqn : y_zero;
+            [ rewrite Z.eqb_eq in y_zero | rewrite Z.eqb_neq in y_zero ].
+          * rewrite y_zero. cbn. lia.
+          * apply (Z.lt_le_trans _ _ _ (bv_unsigned_log2 zero_lt_m)). lia.
+      - apply bv_unsigned_shiftl_nonneg.
+      - apply bv_unsigned_nonneg. }
+Qed.
+
+(** Give the empty bitvector an explicit name to avoid any ambiguity with the notation. *)
+
+Definition bv_empty : bv 0 := 0.
+
+Lemma bv_empty_bits : bv_to_bits bv_empty = [].
+Proof. apply nil_length_inv. rewrite length_bv_to_bits. lia. Qed.
+
+Lemma bv_empty_canonical : ∀ (x : bv 0), x = bv_empty.
+Proof.
+  intros x.
+  destruct x.
+  unfold bv_empty.
+  bv_simplify. f_equal.
+  unfold BvWf, bv_modulus  in bv_is_wf.
+  rewrite Is_true_true, andb_true_iff, Z.ltb_lt, Z.leb_le in bv_is_wf.
+  lia.
+Qed.
+
+(** The empty bitvector is the unit for concatentation. *)
+
+Lemma bv_concat_unit_l : ∀ {n} {x : bv n}, bv_concat n bv_empty x = x.
+Proof.
+  intros n x.
+  rewrite bv_concat_0; [ apply bv_zero_extend_idemp |].
+  destruct x.
+  unfold definitions.bv_unsigned. reflexivity.
+Qed.
+
+Lemma bv_concat_unit_r : ∀ {n} {x : bv n}, bv_concat n x bv_empty = x.
+Proof.
+  intros n x.
+  apply bv_eq.
+  rewrite bv_concat_unsigned'.
+  change (bv_wrap n (Z.lor (bv_unsigned x ≪ Z.of_N 0) (bv_unsigned (bv_0 0))) = bv_unsigned x).
+  rewrite (@bv_0_unsigned 0), Z.lor_0_r, Z.shiftl_0_r.
+  apply bv_wrap_bv_unsigned.
+Qed.
+
+(** Now prove the full [bv_concat_app] lemma. *)
+
+Lemma bv_concat_app : ∀ {n m} {x : bv n} {y : bv m},
+  bv_to_bits (bv_concat (n + m) x y) = bv_to_bits y ++ bv_to_bits x.
+Proof.
+  intros n m x y.
+  destruct (n =? 0)%N eqn : n_zero; [ rewrite N.eqb_eq in n_zero | rewrite N.eqb_neq in n_zero ].
+  - subst.
+    pose proof (bv_empty_canonical x); subst.
+    rewrite bv_empty_bits, bv_concat_unit_l, app_nil_r. reflexivity.
+  - destruct (m =? 0)%N eqn : m_zero; [ rewrite N.eqb_eq in m_zero | rewrite N.eqb_neq in m_zero ].
+    + subst.
+      pose proof (bv_empty_canonical y); subst.
+      rewrite bv_empty_bits, N.add_0_r, bv_concat_unit_r. reflexivity.
+    + apply bv_concat_app_non_empty; lia.
+Qed.
+
+Lemma bool_to_bv_bits : ∀ {b}, bv_to_bits (bool_to_bv 1 b) = [b].
+Proof.
+  intros b.
+  apply (list_eq_same_length _ _ 1).
+  - reflexivity.
+  - rewrite length_bv_to_bits. lia.
+  - intros i lb rb _ L R.
+    rewrite list_lookup_singleton_Some in R. destruct R as [i_zero R].
+    subst.
+    rewrite bv_to_bits_lookup_Some, bool_to_bv_unsigned, bool_to_Z_spec in L; [| lia]. destruct L as [_ L].
+    assert (D : bool_decide (Z.of_nat 0 = 0%Z) = true).
+    { apply bool_decide_eq_true_2. lia. }
+    rewrite D in L.
+    naive_solver.
+Qed.
+
+Lemma bv_concat_cons : ∀ {n b} {x : bv n}, bv_to_bits (bv_concat (N.succ n) x (bool_to_bv 1 b)) = b :: bv_to_bits x.
+Proof.
+  intros n b x.
+  pose proof (@bv_concat_app n 1 x (bool_to_bv 1 b)) as H.
+  rewrite N.add_1_r, bool_to_bv_bits in H.
+  exact H.
+Qed.
+
+Definition bv_cast {n m : N} (E : n = m) (x : bv n) : bv m.
+Proof. rewrite E in x. exact x. Defined.
+
+Module BoolList.
+  (** Convert a list of booleans into a stdpp bitvector. The
+  [bits_to_N] function does this by converting the boolean list into a
+  value of type [N] by traversing the list from left to right, and
+  adding a new least-significant bit to the accumulated value for each
+  element of the list.
+
+  This means it treats a list like <<[true;false;false]>> as the
+  number 4, with the head element being the most significant bit.
+
+  This seems like the most natural way to do it as it avoids any kind
+  of list reversal when converting to the Rocq BinNums-based types. *)
+
+  Definition add_lsb (b : bool) (prefix : option positive) : option positive :=
+    match b with
+    | false =>
+        match prefix with
+        | None => None
+        | Some n => Some (xO n)
+        end
+    | true =>
+        match prefix with
+        | None => Some xH
+        | Some n => Some (xI n)
+        end
+    end.
+
+  Fixpoint bits_to_N (x : list bool) (acc : option positive) : N :=
+    match x with
+    | [] =>
+        match acc with
+        | None => N0
+        | Some n => Npos n
+        end
+    | b :: x => bits_to_N x (add_lsb b acc)
+    end.
+
+  Definition to_Z_unsigned (x : list bool) (prefix : option positive) : Z :=
+    match bits_to_N x prefix with
+    | N0 => Z0
+    | Npos n => Zpos n
+    end.
+
+  Fixpoint positive_to_bits (p : positive) : list bool :=
+    match p with
+    | xH => [true]
+    | xO p => false :: positive_to_bits p
+    | xI p => true :: positive_to_bits p
+    end.
+
+  Definition prefix_to_bits (prefix : option positive) : list bool :=
+    match prefix with
+    | None => []
+    | Some p => positive_to_bits p
+    end.
+
+  Definition prefix_size (prefix : option positive) : nat :=
+    match prefix with
+    | None => 0
+    | Some p => Pos.size_nat p
+    end.
+
+  Lemma Z_pos_size_nat : ∀ {p}, Z.of_N (N.of_nat (Pos.size_nat p)) = Z.pos (Pos.size p).
+  Proof. intros p; induction p; cbn; lia. Qed.
+
+  Lemma pow2_pos_size : ∀ {p}, (Z.pos p < 2 ^ Z.pos (Pos.size p))%Z.
+  Proof.
+    intros p.
+    rewrite Z.log2_lt_pow2; [| lia].
+    induction p; cbn; lia.
+  Qed.
+
+  Lemma to_Z_unsiged_bv_modulus : ∀ {x} prefix,
+    (to_Z_unsigned x prefix < bv_modulus (N.of_nat (prefix_size prefix + length x)))%Z.
+  Proof.
+    intros x.
+    induction x as [| [] x IH]; intros prefix.
+    - destruct prefix; unfold to_Z_unsigned, bv_modulus; cbn; [| lia].
+      rewrite Nat.add_0_r, Z_pos_size_nat.
+      apply pow2_pos_size.
+    - destruct prefix as [p |].
+      + unfold to_Z_unsigned. cbn. fold (to_Z_unsigned x (Some (p~1)%positive)).
+        specialize (IH (Some (p~1)%positive)).
+        apply (Z.lt_le_trans _ _ _ IH).
+        apply bv_modulus_le_mono.
+        rewrite Nat.add_succ_r.
+        reflexivity.
+      + unfold to_Z_unsigned. cbn. fold (to_Z_unsigned x (Some 1%positive)).
+        specialize (IH (Some 1%positive)).
+        apply (Z.lt_le_trans _ _ _ IH).
+        reflexivity.
+    - destruct prefix as [p |].
+      + unfold to_Z_unsigned. cbn. fold (to_Z_unsigned x (Some (p~0)%positive)).
+        specialize (IH (Some (p~0)%positive)).
+        apply (Z.lt_le_trans _ _ _ IH).
+        apply bv_modulus_le_mono.
+        rewrite Nat.add_succ_r.
+        reflexivity.
+      + unfold to_Z_unsigned. cbn. fold (to_Z_unsigned x None).
+        specialize (IH None).
+        apply (Z.lt_le_trans _ _ _ IH).
+        apply bv_modulus_le_mono.
+        cbn. lia.
+  Qed.
+
+  Definition to_bv' (x : list bool) (prefix : option positive) : bv (N.of_nat (prefix_size prefix + length x)) :=
+    Z_to_bv (N.of_nat (prefix_size prefix + length x)) (to_Z_unsigned x prefix).
+
+  (** Now, the actual function that converts a list of booleans to a stdpp bitvector. *)
+
+  Definition to_bv (x : list bool) : bv (N.of_nat (length x)) := to_bv' x None.
+
+  Definition positive_to_bv (p : positive) : bv (N.of_nat (Pos.size_nat p)) :=
+    Z_to_bv (N.of_nat (Pos.size_nat p)) (Z.pos p).
+
+  Lemma pos_app_1 : ∀ {p}, Z.lor (Z.pos p ≪ 1) 1 = Z.pos p~1 .
+  Proof.
+    intros p.
+    rewrite <- shift_equiv.
+    - reflexivity.
+    - lia.
+  Qed.
+
+  Lemma positive_to_bv_concat_1 : ∀ {p}, positive_to_bv p~1 = bv_concat (N.of_nat (S (Pos.size_nat p))) (positive_to_bv p) (1 : bv 1).
+  Proof.
+    intros p.
+    unfold positive_to_bv.
+    bv_simplify. rewrite bv_concat_unsigned'.
+    f_equal. bv_simplify. repeat rewrite bv_wrap_land.
+    cbn.
+    pattern (Z.land (Z.pos p) (Z.ones (Z.of_N (N.of_nat (Pos.size_nat p))))).
+    rewrite Z.land_ones_low.
+    - rewrite Z.land_ones_low; rewrite pos_app_1.
+      + reflexivity.
+      + lia.
+      + destruct p; cbn; repeat (rewrite Nat2N.inj_succ + rewrite N2Z.inj_succ + rewrite Z_pos_size_nat); lia.
+    - lia.
+    - destruct p; cbn; try lia; rewrite Nat2N.inj_succ, N2Z.inj_succ, Z_pos_size_nat; lia.
+  Qed.
+
+  Lemma positive_to_bv_concat_0 : ∀ {p}, positive_to_bv p~0 = bv_concat (N.of_nat (S (Pos.size_nat p))) (positive_to_bv p) (0 : bv 1).
+  Proof.
+    intros p.
+    unfold positive_to_bv.
+    bv_simplify. rewrite bv_concat_unsigned'.
+    f_equal. bv_simplify. repeat rewrite bv_wrap_land.
+    cbn.
+    pattern (Z.land (Z.pos p) (Z.ones (Z.of_N (N.of_nat (Pos.size_nat p))))).
+    rewrite Z.land_ones_low.
+    - rewrite Z.land_ones_low.
+      + reflexivity.
+      + apply Z.shiftl_nonneg; lia.
+      + rewrite Z.log2_shiftl; try lia.
+        destruct p; cbn; repeat (rewrite Nat2N.inj_succ + rewrite N2Z.inj_succ + rewrite Z_pos_size_nat); lia.
+    - lia.
+    - destruct p; cbn; try lia; rewrite Nat2N.inj_succ, N2Z.inj_succ, Z_pos_size_nat; lia.
+  Qed.
+
+  Lemma bool_to_bv_true : bool_to_bv 1 true = 1%bv.
+  Proof.
+    apply bv_eq.
+    rewrite bool_to_bv_unsigned.
+    - bv_simplify. reflexivity.
+    - lia.
+  Qed.
+
+  Lemma bool_to_bv_false : bool_to_bv 1 false = 0%bv.
+  Proof.
+    apply bv_eq.
+    rewrite bool_to_bv_unsigned.
+    - bv_simplify. reflexivity.
+    - lia.
+  Qed.
+
+  Lemma positive_round_trip : ∀ {p},
+    bv_to_bits (positive_to_bv p) = positive_to_bits p.
+  Proof with reflexivity.
+    intros p.
+    induction p as [p IH | p IH |]; cbn.
+    - rewrite positive_to_bv_concat_1, Nat2N.inj_succ, <- bool_to_bv_true, bv_concat_cons, IH...
+    - rewrite positive_to_bv_concat_0, Nat2N.inj_succ, <- bool_to_bv_false, bv_concat_cons, IH...
+    - reflexivity.
+  Qed.
+
+  Lemma prefix_size_add_lsb_Some : ∀ b {p}, prefix_size (add_lsb b (Some p)) = S (prefix_size (Some p)).
+  Proof. intros b prefix; destruct b; try reflexivity. Qed.
+
+  Lemma bv_round_trip' : ∀ {x prefix}, bv_to_bits (to_bv' x prefix) = rev x ++ prefix_to_bits prefix.
+  Proof.
+    intros x.
+    induction x as [| b x IH]; intros prefix.
+    - destruct prefix as [prefix |]; try reflexivity.
+      cbn. rewrite <- positive_round_trip.
+      unfold to_bv', positive_to_bv. cbn. rewrite Nat.add_0_r. reflexivity.
+    - destruct prefix as [p |].
+      + unfold to_bv', to_Z_unsigned. cbn [bits_to_N].
+        fold (to_Z_unsigned x (add_lsb b (Some p))).
+        rewrite length_cons, <- Nat.add_succ_comm. rewrite <- (prefix_size_add_lsb_Some b).
+        fold (to_bv' x (add_lsb b (Some p))).
+        rewrite IH.
+        destruct b; cbn; rewrite <- app_assoc; reflexivity.
+      + destruct b.
+        * unfold to_bv', to_Z_unsigned. cbn [bits_to_N add_lsb].
+          fold (to_Z_unsigned x (Some 1%positive)).
+          rewrite length_cons, <- Nat.add_succ_comm.
+          replace (S (prefix_size None)) with (prefix_size (Some 1%positive)) by reflexivity.
+          fold (to_bv' x (Some 1%positive)).
+          rewrite IH.
+          cbn; rewrite <- app_assoc; reflexivity.
+        * specialize (IH None).
+          cbn in *. rewrite app_nil_r in *.
+          rewrite <- IH, <- bool_to_bv_bits, <- bv_concat_app.
+          (* Implicit arguments for bv_to_bits are different *)
+          rewrite N.add_1_l, <- Nat2N.inj_succ; f_equal.
+          bv_simplify; f_equal.
+          rewrite bv_zero_extend_unsigned; [| lia ].
+          unfold to_bv'. cbn.
+          repeat rewrite Z_to_bv_small; try reflexivity.
+          ** split.
+          *** unfold to_Z_unsigned; destruct_match; lia.
+          *** apply (to_Z_unsiged_bv_modulus None).
+          ** split.
+          *** unfold to_Z_unsigned; destruct_match; lia.
+          *** apply (Z.lt_le_trans _ _ _ (to_Z_unsiged_bv_modulus None)). reflexivity.
+  Qed.
+
+  Lemma bv_round_trip : ∀ {x}, rev (bv_to_bits (to_bv x)) = x.
+  Proof.
+    intros x.
+    unfold to_bv.
+    pose proof (@bv_round_trip' x None) as H.
+    cbn in H. rewrite H, app_nil_r.
+    apply rev_involutive.
+  Qed.
+End BoolList.
